theories/aps_plus_1/examples/list_length.v
@@ -10,38 +10,53 @@ From simuliris.aps_plus_1 Require Import
   soundness.
 
 Definition list_length : data_human_program := {[
-  "list_length" := (BNamed "arg", (
-    match: ![𝟙] "arg" with
-      NIL =>
-        0
-    | CONS <>, "xs" =>
-        1 + $"list_length" "xs"
-    end
-  )%data_human_expr)
+  "list_length" :=
+    {|data_human_definition_annot :=
+        [] ;
+      data_human_definition_param :=
+        BNamed "arg" ;
+      data_human_definition_body :=
+        match: ![𝟙] "arg" with
+          NIL =>
+            0
+        | CONS <>, "xs" =>
+            1 + $"list_length" "xs"
+        end ;
+    |}
 ]}.
 
 Definition list_length_aps_plus : data_human_program := {[
-  "list_length" := (BNamed "arg", (
-    match: ![𝟙] "arg" with
-      NIL =>
-        0
-    | CONS "<>", "xs" =>
-        let: "arg" := "xs" in
-        $"list_length_aps" (1, "arg")
-    end
-  )%data_human_expr) ;
-  "list_length_aps" := (BNamed "arg", (
-    let: "acc" := ![𝟙] "arg" in
-    let: "arg" := ![𝟚] "arg" in
-    match: ![𝟙] "arg" with
-      NIL =>
-      "acc" + 0
-    | CONS "<>", "xs" =>
-        let: "acc" := "acc" + 1 in
-        let: "arg" := "xs" in
-        $"list_length_aps" ("acc", "arg")
-    end
-  )%data_human_expr)
+  "list_length" :=
+    {|data_human_definition_annot :=
+        [] ;
+      data_human_definition_param :=
+        BNamed "arg" ;
+      data_human_definition_body :=
+        match: ![𝟙] "arg" with
+          NIL =>
+            0
+        | CONS "<>", "xs" =>
+            let: "arg" := "xs" in
+            $"list_length_aps" (1, "arg")
+        end ;
+    |} ;
+  "list_length_aps" :=
+    {|data_human_definition_annot :=
+        [] ;
+      data_human_definition_param :=
+        BNamed "arg" ;
+      data_human_definition_body :=
+        let: "acc" := ![𝟙] "arg" in
+        let: "arg" := ![𝟚] "arg" in
+        match: ![𝟙] "arg" with
+          NIL =>
+          "acc" + 0
+        | CONS "<>", "xs" =>
+            let: "acc" := "acc" + 1 in
+            let: "arg" := "xs" in
+            $"list_length_aps" ("acc", "arg")
+        end ;
+    |}
 ]}.
 
 Lemma list_length_aps_plus_sound :
@@ -56,9 +71,9 @@ Proof.
     + apply data_human_program_compile_scoped.
   - rewrite /data_human_program_compile map_fmap_singleton fmap_insert map_fmap_singleton /=.
     exists {["list_length" := "list_length_aps"]}; try set_solver.
-    + intros * (<- & <-)%lookup_singleton_Some.
+    + intros * (<- & <-)%lookup_singleton_Some ->.
       rewrite lookup_insert.
       eexists. split; last done. repeat econstructor.
-    + intros * (<- & <-)%lookup_singleton_Some (_ & <-)%lookup_singleton_Some.
+    + intros * (<- & <-)%lookup_singleton_Some -> (_ & <-)%lookup_singleton_Some.
       eexists. split; last done. repeat econstructor.
 Qed.
