theories/aps_plus_2/examples/list_sum.v
@@ -10,39 +10,54 @@ From simuliris.aps_plus_2 Require Import
   definition.
 
 Definition list_sum : data_human_program := {[
-  "list_sum" := (BNamed "arg", (
-    match: ![𝟙] "arg" with
-      NIL =>
-        0
-    | CONS "x", "xs" =>
-        "x" + $"list_sum" "xs"
-    end
-  )%data_human_expr)
+  "list_sum" :=
+    {|data_human_definition_annot :=
+        [] ;
+      data_human_definition_param :=
+        BNamed "arg" ;
+      data_human_definition_body :=
+        match: ![𝟙] "arg" with
+          NIL =>
+            0
+        | CONS "x", "xs" =>
+            "x" + $"list_sum" "xs"
+        end ;
+    |}
 ]}.
 
 Definition list_sum_aps_plus : data_human_program := {[
-  "list_sum" := (BNamed "arg", (
-    match: ![𝟙] "arg" with
-      NIL =>
-        0
-    | CONS "x", "xs" =>
-        let: "acc" := "x" in
-        let: "arg" := "xs" in
-        $"list_sum_aps" ("acc", "arg")
-    end
-  )%data_human_expr) ;
-  "list_sum_aps" := (BNamed "arg", (
-    let: "acc" := ![𝟙] "arg" in
-    let: "arg" := ![𝟚] "arg" in
-    match: ![𝟙] "arg" with
-      NIL =>
-        0 + "acc"
-    | CONS "x", "xs" =>
-        let: "acc" := "x" + "acc" in
-        let: "arg" := "xs" in
-        $"list_sum_aps" ("acc", "arg")
-    end
-  )%data_human_expr)
+  "list_sum" :=
+    {|data_human_definition_annot :=
+        [] ;
+      data_human_definition_param :=
+        BNamed "arg" ;
+      data_human_definition_body :=
+        match: ![𝟙] "arg" with
+          NIL =>
+            0
+        | CONS "x", "xs" =>
+            let: "acc" := "x" in
+            let: "arg" := "xs" in
+            $"list_sum_aps" ("acc", "arg")
+        end ;
+    |} ;
+  "list_sum_aps" :=
+    {|data_human_definition_annot :=
+        [] ;
+      data_human_definition_param :=
+        BNamed "arg" ;
+      data_human_definition_body :=
+        let: "acc" := ![𝟙] "arg" in
+        let: "arg" := ![𝟚] "arg" in
+        match: ![𝟙] "arg" with
+          NIL =>
+            0 + "acc"
+        | CONS "x", "xs" =>
+            let: "acc" := "x" + "acc" in
+            let: "arg" := "xs" in
+            $"list_sum_aps" ("acc", "arg")
+        end ;
+    |}
 ]}.
 
 Section list_sum_aps_plus_sound.
@@ -63,10 +78,10 @@ Section list_sum_aps_plus_sound.
       + apply data_human_program_compile_scoped.
     - rewrite /data_human_program_compile map_fmap_singleton fmap_insert map_fmap_singleton /=.
       exists {["list_sum" := "list_sum_aps"]}; try set_solver.
-      + intros * (<- & <-)%lookup_singleton_Some.
+      + intros * (<- & <-)%lookup_singleton_Some ->.
         rewrite lookup_insert.
         eexists. split; last done. repeat econstructor.
-      + intros * (<- & <-)%lookup_singleton_Some (_ & <-)%lookup_singleton_Some.
+      + intros * (<- & <-)%lookup_singleton_Some -> (_ & <-)%lookup_singleton_Some.
         eexists. split; last done. repeat econstructor.
   Qed.
 End list_sum_aps_plus_sound.
