theories/inline/soundness.v
@@ -34,8 +34,8 @@ Section sim_GS.
       vₛ' ≈ vₜ' -∗
       Ψ vₛ' vₜ'.
   Definition inline_protocol_inline Ψ eₛ eₜ : iProp Σ :=
-    ∃ func annot e_funcₛ e_funcₜ vₛ vₜ,
-    ⌜sim_progₛ !! func = Some e_funcₛ ∧ inline_expr sim_progₛ e_funcₛ e_funcₜ⌝ ∗
+    ∃ func annot defₛ e_funcₛ e_funcₜ vₛ vₜ,
+    ⌜sim_progₛ !! func = Some defₛ ∧ e_funcₛ = defₛ.(data_definition_body) ∧ inline_expr sim_progₛ e_funcₛ e_funcₜ⌝ ∗
     ⌜eₛ = (DataFunc func annot) vₛ ∧ eₜ = (let: vₜ in e_funcₜ)%data_expr⌝ ∗
     vₛ ≈ vₜ ∗
       ∀ vₛ' vₜ',
@@ -59,7 +59,7 @@ Section sim_GS.
       |
       | * Hinline1 IH1 Hinline2 IH2
       | * Hinline1 IH1 Hinline2 IH2
-      | * Hfunc Hinline_func IHfunc Hinline IH
+      | * Hfunc -> Hinline_func IHfunc Hinline IH
       | * Hinline IH
       | * Hinline1 IH1 Hinline2 IH2
       |
@@ -87,7 +87,7 @@ Section sim_GS.
       sim_apply (IH with "[//] [HΦ]"); first auto with data_lang.
       iIntros "%vₛ %vₜ #Hv".
       iApply (sim_apply_protocol _ (sim_post_vals' (≈))). iIntros "%σₛ %σₜ $ !>". iSplitR.
-      { iRight. iExists func, annot, e_funcₛ, e_funcₜ, vₛ, vₜ. repeat iSplit; try iSmash.
+      { iRight. repeat iExists _. repeat iSplit; try iSmash.
         - iPureIntro.
           rewrite (subst_data_expr_scoped_1 _ ids); asimpl; try done.
           eapply data_expr_scoped_inline; naive_solver.
@@ -127,20 +127,21 @@ Section sim_GS.
     eapply data_program_scoped_inline in Hprogₛ_scoped as Hprogₜ_scoped; last done.
     iApply sim_close_pure_head_step. clear eₛ eₜ. iIntros "!> %Ψ %eₛ %eₜ [Hprotocol | Hprotocol]".
     - iDestruct "Hprotocol" as "(%func & %annot & %vₛ & %vₜ & %Hfuncₛ & (-> & ->) & #Hv & HΨ)".
-      simpl in Hfuncₛ. apply lookup_lookup_total_dom in Hfuncₛ. set (eₛ := _ !!! _) in Hfuncₛ.
-      edestruct inline.(inline_transform) as (eₜ & Hdir & Hfuncₜ); first done.
-      iExists eₛ.[#vₛ/], eₜ.[#vₜ/]. iSplit; first auto with data_lang.
-      erewrite (subst_data_program_scoped' ids inhabitant.ₛ#); last done; last done.
-      erewrite (subst_data_program_scoped' ids inhabitant.ₜ#); last done; last done.
+      simpl in Hfuncₛ. apply lookup_lookup_total_dom in Hfuncₛ.
+      set defₛ := _ !!! _ in Hfuncₛ. set eₛ := defₛ.(data_definition_body).
+      edestruct inline.(inline_transform) as (eₜ & Hdir & Hfuncₜ); [done.. |].
+      iExists _, _. iSplit; first eauto 10 with data_lang. sim_asimpl.
+      erewrite (subst_data_program_scoped' ids inhabitant.ₛ# _ sim_progₛ); [| done..].
+      erewrite (subst_data_program_scoped' ids inhabitant.ₜ# _ sim_progₜ); [| done..].
       iDestruct (inline_specification $! (≈)%I with "[//] [] [//] []") as "Hsim"; eauto.
       + iApply (bisubst_cons_well_formed with "Hv").
         iApply bisubst_inhabitant_well_formed.
       + rewrite -bisubst_consₛ -bisubst_consₜ.
         sim_mono "Hsim". rewrite sim_post_vals_unseal. iSmash.
-    - iDestruct "Hprotocol" as "(%func & %annot & %e_funcₛ & %e_funcₜ & %vₛ & %vₜ & (%Hfunc & %Hinline_func) & (-> & ->) & #Hv & HΨ)".
-      iExists _, _. iSplit; first auto with data_lang.
+    - iDestruct "Hprotocol" as "(%func & %annot & %defₛ & %e_funcₛ & %e_funcₜ & %vₛ & %vₜ & (%Hfunc & -> & %Hinline_func) & (-> & ->) & #Hv & HΨ)".
+      iExists _, _. iSplit; first eauto 10 with data_lang.
       iDestruct (inline_specification $! (≈)%I with "[//] []") as "Hsim"; [auto with data_lang.. | naive_solver | iSmash |].
-      erewrite (subst_data_program_scoped' _ inhabitant.ₛ#); last done; last done.
+      erewrite (subst_data_program_scoped' ids inhabitant.ₛ# _ sim_progₛ); [| done..].
       rewrite (subst_data_expr_scoped_1' _ inhabitant.ₜ# vₜ); last first.
       { eapply data_expr_scoped_inline; [| done |]; naive_solver. }
       erewrite bisubst_consₛ, bisubst_consₜ.
