theories/tmc/examples/list_append.v
@@ -10,50 +10,65 @@ From simuliris.tmc Require Import
   soundness.
 
 Definition list_append : data_human_program := {[
-  "list_append" := (BNamed "arg", (
-    let: "xs" := ![𝟙] "arg" in
-    let: "ys" := ![𝟚] "arg" in
-    match: "xs" with
-      NIL =>
-        NILₕ
-    | CONS "x", "xs" =>
-        CONSₕ "x" ($"list_append" ("xs", "ys"))
-    end
-  )%data_human_expr)
+  "list_append" :=
+    {|data_human_definition_annot :=
+        [] ;
+      data_human_definition_param :=
+        BNamed "arg" ;
+      data_human_definition_body :=
+        let: "xs" := ![𝟙] "arg" in
+        let: "ys" := ![𝟚] "arg" in
+        match: "xs" with
+          NIL =>
+            NILₕ
+        | CONS "x", "xs" =>
+            CONSₕ "x" ($"list_append" ("xs", "ys"))
+        end ;
+    |}
 ]}.
 
 Definition list_append_tmc : data_human_program := {[
-  "list_append" := (BNamed "arg", (
-    let: "xs" := ![𝟙] "arg" in
-    let: "ys" := ![𝟚] "arg" in
-    match: "xs" with
-      NIL =>
-        NILₕ
-    | CONS "x", "xs" =>
-        let: "dst" := CONSₕ "x" #ₕ() in
-        ( let: "arg" := ("xs", "ys") in
-          $"list_append_dps" ("dst", 𝟚, "arg")
-        ) ;;
-        "dst"
-    end
-  )%data_human_expr) ;
-  "list_append_dps" := (BNamed "arg", (
-    let: "dst_idx" := ![𝟙] "arg" in
-    let: "idx" := ![𝟚] "dst_idx" in
-    let: "dst" := ![𝟙] "dst_idx" in
-    let: "arg" := ![𝟚] "arg" in
-    let: "xs" := ![𝟙] "arg" in
-    let: "ys" := ![𝟚] "arg" in
-    match: "xs" with
-      NIL =>
-      "dst" <-["idx"]- NILₕ
-    | CONS "x", "xs" =>
-        let: "dst'" := CONSₕ "x" #ₕ() in
-        "dst" <-["idx"]- "dst'" ;;
-        let: "arg" := ("xs", "ys") in
-        $"list_append_dps" ("dst'", 𝟚, "arg")
-    end
-  )%data_human_expr)
+  "list_append" :=
+    {|data_human_definition_annot :=
+        [] ;
+      data_human_definition_param :=
+        BNamed "arg" ;
+      data_human_definition_body :=
+        let: "xs" := ![𝟙] "arg" in
+        let: "ys" := ![𝟚] "arg" in
+        match: "xs" with
+          NIL =>
+            NILₕ
+        | CONS "x", "xs" =>
+            let: "dst" := CONSₕ "x" #ₕ() in
+            ( let: "arg" := ("xs", "ys") in
+              $"list_append_dps" ("dst", 𝟚, "arg")
+            ) ;;
+            "dst"
+        end ;
+    |} ;
+  "list_append_dps" :=
+    {|data_human_definition_annot :=
+        [] ;
+      data_human_definition_param :=
+        BNamed "arg" ;
+      data_human_definition_body :=
+        let: "dst_idx" := ![𝟙] "arg" in
+        let: "idx" := ![𝟚] "dst_idx" in
+        let: "dst" := ![𝟙] "dst_idx" in
+        let: "arg" := ![𝟚] "arg" in
+        let: "xs" := ![𝟙] "arg" in
+        let: "ys" := ![𝟚] "arg" in
+        match: "xs" with
+          NIL =>
+          "dst" <-["idx"]- NILₕ
+        | CONS "x", "xs" =>
+            let: "dst'" := CONSₕ "x" #ₕ() in
+            "dst" <-["idx"]- "dst'" ;;
+            let: "arg" := ("xs", "ys") in
+            $"list_append_dps" ("dst'", 𝟚, "arg")
+        end ;
+    |}
 ]}.
 
 Lemma list_append_tmc_sound :
@@ -68,10 +83,10 @@ Proof.
     + apply data_human_program_compile_scoped.
   - rewrite /data_human_program_compile map_fmap_singleton fmap_insert map_fmap_singleton /=.
     exists {["list_append" := "list_append_dps"]}; try set_solver.
-    + intros * (<- & <-)%lookup_singleton_Some.
+    + intros * (<- & <-)%lookup_singleton_Some ->.
       rewrite lookup_insert.
       eexists. split; last done. repeat econstructor.
-    + intros * (<- & <-)%lookup_singleton_Some (_ & <-)%lookup_singleton_Some.
+    + intros * (<- & <-)%lookup_singleton_Some -> (_ & <-)%lookup_singleton_Some.
       eexists. split; last done. repeat constructor.
       eapply tmc_dps_constr_1; first constructor.
       * eapply tmc_dps_call; repeat constructor.
